cava/arrow-examples/Aes/unrolled_cipher.v
@@ -18,7 +18,7 @@ From Coq Require Import Arith Eqdep_dec Vector Lia NArith Omega String Ndigits.
 From Arrow Require Import Category Arrow.
 From Cava Require Import Arrow.ArrowExport BitArithmetic.
 
-From ArrowExamples Require Import Combinators Aes.pkg Aes.mix_columns Aes.sub_bytes Aes.shift_rows.
+From ArrowExamples Require Import Combinators Aes.pkg Aes.mix_columns Aes.sbox Aes.sub_bytes Aes.shift_rows.
 
 Import VectorNotations.
 Import KappaNotation.
@@ -39,35 +39,162 @@ Definition cipher_round
     !(map2 <[ !(map2 <[\x y => x ^ y]>) ]> ) stage3 stage_key 
     ]>.
 
-Definition initial_round_constant
+(* Note: aes_key_expand in OpenTitan is stateful, this version is not *)
+Program Definition aes_key_expand
+  (sbox_impl: SboxImpl)
   : forall cava: Cava, 
-    << Bit, Unit >> ~> Vector (Vector Bit 8) 4 :=
-  <[ \op_i =>
-    #0 :: #0 :: #0 :: (
-    if op_i == !CIPH_FWD 
-    then # 1
-    else #64)
-    :: []
-    ]>.
- 
-    (* rcon_d = 
-    (op_i == CIPH_FWD) ? aes_mul2(rcon_q) :
-    (op_i == CIPH_INV) ? aes_div2(rcon_q) : 8'h01;  *)
-Definition increase_round_constant
-  : forall cava: Cava, 
-    << Bit, Vector Bit 8, Unit >> ~> Vector Bit 8 :=
-  <[ \op_i x =>
-    if op_i == !CIPH_FWD 
-    then !aes_mul2 x
-    else !aes_div2 x
-    ]>.
-
-Definition unrolled_cipher
-  : forall cava: Cava, 
-    <<Bit
-    , Vector (Vector (Vector Bit 8) 4) 4 (* data *)
-    , Vector (Vector (Vector Bit 8) 4) 4 (* key *)
+    << Bit (* op_i *)
+    , Vector Bit 3 (* round id *)
+    , Vector Bit 8 (* rcon input *)
+    , Vector (Vector (Vector Bit 8) 4) 8 (* input key *)
     , Unit
     >> ~> 
-      Vector (Vector (Vector Bit 8) 4) 4 :=
-  <[\op_i data_i _ => data_i ]>.
+      << Vector Bit 8, Vector (Vector (Vector Bit 8) 4) 8>> :=
+  let sbox := curry (aes_sbox sbox_impl) in
+  let mapped_sbox := <[ !(map sbox) ]> in
+  <[\op_i round_id rcon key_i => 
+    (* if (key_len_i == AES_256 && rnd[0] == 1'b0) begin
+    use_rcon = 1'b0;
+    end *)
+    let use_rcon = round_id[#0] in
+
+    (* rcon_d = (op_i == CIPH_FWD) ? aes_mul2(rcon_q) :
+                (op_i == CIPH_INV) ? aes_div2(rcon_q) : 8'h01; *)
+    let rcon = 
+      if round_id == #0
+      then 
+        if op_i == !CIPH_FWD
+        then #1
+        else #64
+      else 
+        if op_i == !CIPH_FWD
+        then !aes_mul2 rcon
+        else !aes_div2 rcon in
+
+    (* AES_256: begin
+      unique case (op_i)
+        CIPH_FWD: rot_word_in = key_i[7];
+        CIPH_INV: rot_word_in = key_i[3];
+        default:  rot_word_in = key_i[7]; *)
+    let rot_word_in = 
+      if op_i == !CIPH_FWD
+      then key_i[#7]
+      else key_i[#3] in
+
+    (* assign rot_word_out = aes_circ_byte_shift(rot_word_in, 2'h3); *)
+    let rot_word_out = !aes_circ_byte_shift rot_word_in #3 in
+
+    (* assign sub_word_in = use_rot_word ? rot_word_out : rot_word_in; *)
+    let sub_word_in = 
+      if use_rcon (* for AES_256 use_rcon == use_rot_word *)
+      then rot_word_out
+      else rot_word_in in
+
+    let sub_word_out = !mapped_sbox (!(map2 <[\x y => (x,y)]>) (!replicate op_i) sub_word_in) in
+    let sub_word_out_flat = !flatten sub_word_out in
+
+    (* assign rcon_add_in  = sub_word_out[7:0]; *)
+    let rcon_add_in = sub_word_out_flat[:7:0] in
+    (* assign rcon_add_out = rcon_add_in ^ rcon_q; *)
+    let rcon_add_out = rcon_add_in ^ rcon in
+    (* assign rcon_added   = {sub_word_out[31:8], rcon_add_out}; *)
+    let rcon_added   = concat rcon_add_out sub_word_out_flat[:31:8] in
+
+    (* // Mux output coming from Rcon & SubWord
+    assign irregular = use_rcon ? rcon_added : sub_word_out; *)
+    let irregular = if use_rcon then rcon_added else sub_word_out_flat in
+
+    (* AES_256: begin
+        unique case (op_i)
+          CIPH_FWD: begin
+            if (rnd == 0) begin
+              // Round 0: Nothing to be done
+              // The Full Key registers are not updated
+              regular = {key_i[3:0], key_i[7:4]};
+            end else begin
+              // Shift down old upper half
+              regular[3:0] = key_i[7:4];
+              // Generate new upper half
+              regular[4]   = irregular ^ key_i[0];
+              for (int i=1; i<4; i++) begin
+                regular[i+4] = regular[i+4-1] ^ key_i[i];
+              end
+            end // rnd == 0
+          end
+
+        endcase
+      end *)
+    let regular =
+      if round_id == #0
+      then concat key_i[:7:4] key_i[:3:0] 
+      else 
+        if op_i == !CIPH_FWD
+        then 
+          (* todo: this is a "scan" op *)
+          let regular_4 = (!reshape irregular) ^ key_i[#0] in
+          let regular_5 = regular_4 ^ key_i[#1] in
+          let regular_6 = regular_5 ^ key_i[#2] in
+          let regular_7 = regular_6 ^ key_i[#3] in
+          snoc (snoc (snoc (snoc key_i[:7:4] regular_4) regular_5) regular_6) regular_7
+
+          (* CIPH_INV: begin
+            if (rnd == 0) begin
+              // Round 0: Nothing to be done
+              // The Full Key registers are not updated
+              regular = {key_i[3:0], key_i[7:4]};
+            end else begin
+              // Shift up old lower half
+              regular[7:4] = key_i[3:0];
+              // Generate new lower half
+              regular[0]   = irregular ^ key_i[4];
+              for (int i=0; i<3; i++) begin
+                regular[i+1] = key_i[4+i] ^ key_i[4+i+1];
+              end
+            end // rnd == 0
+          end *)
+        else 
+          let regular_0 = (!reshape irregular) ^ key_i[#4] in
+          let regular_1 = key_i[#4] ^ key_i[#5] in
+          let regular_2 = key_i[#5] ^ key_i[#6] in
+          let regular_3 = key_i[#6] ^ key_i[#7] in
+          cons regular_0 (cons regular_1 (cons regular_2 (cons regular_3 key_i[:3:0])))
+      in
+    (rcon, regular)
+    ]>.
+Next Obligation. lia. Defined.
+Next Obligation. lia. Defined. 
+Next Obligation. lia. Defined.
+Next Obligation. lia. Defined.
+Next Obligation. lia. Defined.
+
+(* stateless *)
+Program Definition unrolled_foward_cipher
+  (sbox_impl: SboxImpl)
+  : forall cava: Cava, 
+    <<
+      Vector Bit 8 (* rcon *)
+    , Vector (Vector (Vector Bit 8) 4) 4 (* data *)
+    , Vector (Vector (Vector Bit 8) 4) 8 (* key *)
+    , Unit
+    >> ~> 
+    << 
+      Vector Bit 8 (* rcon *)
+    , Vector (Vector (Vector Bit 8) 4) 4 (* data *)
+    , Vector (Vector (Vector Bit 8) 4) 8 (* key state *)
+    >>
+      :=
+  let cipher_round := cipher_round sbox_impl in  
+  let aes_key_expand := aes_key_expand sbox_impl in  
+  <[\rcon data_i key => 
+    let round = #0 in
+    let rcon = #1 in
+
+    let key_words_0 = key[:3:0] in
+    let key_bytes_0 = !aes_transpose key_words_0 in
+    let round_key = key_bytes_0 in
+
+    let '(rcon, new_key) = !aes_key_expand !CIPH_FWD round rcon key in
+
+    (rcon, !cipher_round !CIPH_FWD data_i round_key, new_key)
+    ]>.
+Next Obligation. lia. Defined.
